tidy, use lazy/eager_step_split as defn instead

isabelle/Distinct_Elems_Analysis.thy
@@ -8,13 +8,42 @@ imports
   CVM.Distinct_Elems_Nondet
 begin
 
-context with_threshold
-begin
+sledgehammer_params [
+  (* verbose *)
+  minimize = true,
+  preplay_timeout = 15,
+  timeout = 60,
+  max_facts = smart,
+  provers = "
+    cvc4 z3 verit
+    e vampire spass
+  "
+]
 
-context
+locale with_threshold_and_eps = with_threshold +
   fixes \<epsilon> :: real
   assumes eps_pos : \<open>\<epsilon> > 0\<close>
 begin
+
+lemma estimation_error_1_sided:
+  assumes "finite X"
+  shows
+    "measure_pmf.prob
+    (binomial_pmf (card X) (1 / 2 ^ (K::nat)))
+    {t. t \<ge> n} \<le> foo"
+  sorry
+
+abbreviation beyond_eps_range_of_card :: \<open>'a list \<Rightarrow> nat \<Rightarrow> bool\<close> where
+  \<open>beyond_eps_range_of_card xs n \<equiv> real n >[\<epsilon>] card (set xs)\<close>
+
+lemma estimation_error_2_sided:
+  assumes "finite X"
+  assumes "\<epsilon> > 0"
+  shows
+    "measure_pmf.prob
+    (binomial_pmf (card X) (1 / 2 ^ (K::nat)))
+    {t. beyond_eps_range_of_card xs t} \<le> bar"
+  sorry
 
 lemma estimate_distinct_errror_bound_fail_2:
   shows "\<P>(st in
@@ -76,7 +105,7 @@ lemma estimate_distinct_errror_bound_L_binom:
        (run_reader (eager_algorithm xs))
        (fair_bernoulli_matrix (length xs) (length xs))).
     state_k st \<le> L \<and>
-      beyond_eps_range_of_card \<epsilon> xs (compute_estimate st))
+      beyond_eps_range_of_card xs (compute_estimate st))
     \<le> foo (card (set xs)) L" (is "?L \<le> ?R")
 proof -
   (* Splits the error event for k=0, k=1,...,k=L *)
@@ -88,7 +117,7 @@ proof -
        (run_reader (eager_algorithm xs))
        (fair_bernoulli_matrix (length xs) (length xs))).
       state_k st = q \<and>
-      beyond_eps_range_of_card \<epsilon> xs (compute_estimate st)))
+      beyond_eps_range_of_card xs (compute_estimate st)))
    {0..L}" sorry
   (* Now we go into nondeterministic *)
   also have "... \<le>
@@ -97,7 +126,7 @@ proof -
     \<P>(X in
       (map_pmf (nondet_alg_aux q xs)
          (fair_bernoulli_matrix (length xs) (length xs))).
-      beyond_eps_range_of_card \<epsilon> xs (card X * 2 ^ q)))
+      beyond_eps_range_of_card xs (card X * 2 ^ q)))
    {0..L}"
     sorry
   (* Go into Binomial then use Chernoff *)
@@ -112,7 +141,7 @@ lemma estimate_distinct_error_bound:
   assumes "(L::nat) = undefined"
   shows "
     \<P>(n in estimate_distinct xs.
-      n |> fail_or_satisfies (beyond_eps_range_of_card \<epsilon> xs))
+      n |> fail_or_satisfies (beyond_eps_range_of_card xs))
      \<le> real (length xs) / 2 ^ threshold + bar \<epsilon> thresh"
   (is "?L \<le> ?R")
 proof -
@@ -127,13 +156,13 @@ proof -
 
   have "?L \<le> real (length xs) / 2 ^ threshold
     + \<P>(n in estimate_distinct_no_fail xs.
-       n |> (beyond_eps_range_of_card \<epsilon> xs))"
+       n |> (beyond_eps_range_of_card xs))"
     by (intro prob_estimate_distinct_fail_or_satisfies_le)
   
   moreover have "... =
     real (length xs) / 2 ^ threshold
       + \<P>(st in ?E.
-        beyond_eps_range_of_card \<epsilon> xs (compute_estimate st))"
+        beyond_eps_range_of_card xs (compute_estimate st))"
     unfolding *
     by auto
   moreover have "... \<le>
@@ -141,14 +170,12 @@ proof -
       + \<P>(st in ?E. state_k st > L)
       + \<P>(st in ?E. 
         state_k st \<le> L \<and>
-          beyond_eps_range_of_card \<epsilon> xs (compute_estimate st))"
+          beyond_eps_range_of_card xs (compute_estimate st))"
     by (auto intro!: pmf_add)
  
   ultimately show ?thesis
     sorry
 qed
-
-end
 
 end
 
